ReactorModel/Execution/Theorems/Step/Skip.lean
@@ -7,7 +7,7 @@ namespace Execution.Step.Skip
 
 variable [Hierarchical α] {s₁ : State α}
 
-def rcn :                      (s₁ ↓ₛ s₂) → ID                   | mk (rcn := rcn) .. => rcn
+def rcn :                      (s₁ ↓ₛ s₂) → α✦                   | mk (rcn := rcn) .. => rcn
 theorem allows_rcn :       (e : s₁ ↓ₛ s₂) → Allows s₁ e.rcn      | mk a _ => a
 theorem not_triggers_rcn : (e : s₁ ↓ₛ s₂) → ¬Triggers s₁ e.rcn   | mk _ t => t
 theorem dst_eq :           (e : s₁ ↓ₛ s₂) → s₂ = s₁.record e.rcn | mk .. => rfl
@@ -25,29 +25,29 @@ theorem equiv (e : s₁ ↓ₛ s₂) : s₁.rtr ≈ s₂.rtr := by
   simp [e.dst_eq, State.record_preserves_rtr]
   exact .refl _
 
-theorem progress_eq (e : s₁ ↓ₛ s₂) : s₂.progress = s₁.progress.insert e.rcn := by 
+theorem progress_eq (e : s₁ ↓ₛ s₂) : s₂.progress = s₁.progress.insert e.rcn := by
   simp [e.dst_eq, State.record_progress_eq]
 
 theorem preserves_nontrivial {e : s₁ ↓ₛ s₂} (n : s₁.Nontrivial) : s₂.Nontrivial :=
   n.equiv e.equiv
 
-theorem indep_allows_iff (e : s₁ ↓ₛ s₂) (hi : i ≮[s₁.rtr]≯ e.rcn) : 
+theorem indep_allows_iff (e : s₁ ↓ₛ s₂) (hi : i ≮[s₁.rtr]≯ e.rcn) :
     s₁.Allows i ↔ s₂.Allows i := by
   simp [e.dst_eq, Allows.iff_record_indep hi.symm]
 
-theorem triggers_iff (e : s₁ ↓ₛ s₂) : 
+theorem triggers_iff (e : s₁ ↓ₛ s₂) :
     s₁.Triggers i ↔ s₂.Triggers i := by
   simp [e.dst_eq, Triggers.iff_record (s := s₁) (i₁ := e.rcn)]
 
-theorem comm 
-    (e₁ : s ↓ₛ s₁) (e₁₂ : s₁ ↓ₛ s₁₂) (e₂ : s ↓ₛ s₂) (e₂₁ : s₂ ↓ₛ s₂₁) (hr₁ : e₁.rcn = e₂₁.rcn) 
-    (hr₂ : e₂.rcn = e₁₂.rcn) : s₁₂ = s₂₁ := by 
+theorem comm
+    (e₁ : s ↓ₛ s₁) (e₁₂ : s₁ ↓ₛ s₁₂) (e₂ : s ↓ₛ s₂) (e₂₁ : s₂ ↓ₛ s₂₁) (hr₁ : e₁.rcn = e₂₁.rcn)
+    (hr₂ : e₂.rcn = e₁₂.rcn) : s₁₂ = s₂₁ := by
   ext1
-  case rtr => 
-    exact e₁₂.preserves_rtr ▸ e₁.preserves_rtr ▸ e₂₁.preserves_rtr ▸ e₂.preserves_rtr 
-  case tag => 
+  case rtr =>
+    exact e₁₂.preserves_rtr ▸ e₁.preserves_rtr ▸ e₂₁.preserves_rtr ▸ e₂.preserves_rtr
+  case tag =>
     exact e₁₂.preserves_tag ▸ e₁.preserves_tag ▸ e₂₁.preserves_tag ▸ e₂.preserves_tag
-  case events => 
+  case events =>
     exact e₁₂.preserves_events ▸ e₁.preserves_events ▸ e₂₁.preserves_events ▸ e₂.preserves_events
   case progress  =>
     have h₁ := e₁.progress_eq ▸ e₁₂.progress_eq
@@ -61,8 +61,8 @@ theorem unprocessed_eq (e : s₁ ↓ₛ s₂) : s₂.unprocessed = s₁.unproces
   simp [State.unprocessed, Equivalent.obj?_rcn_eq e.equiv, and_assoc, e.progress_eq]
   intro _; simp [Set.insert]; push_neg; simp [and_comm]
 
-theorem rcn_mem_unprocessed (e : s₁ ↓ₛ s₂) : e.rcn ∈ s₁.unprocessed := 
-  ⟨e.allows_rcn.mem, e.allows_rcn.unprocessed⟩ 
+theorem rcn_mem_unprocessed (e : s₁ ↓ₛ s₂) : e.rcn ∈ s₁.unprocessed :=
+  ⟨e.allows_rcn.mem, e.allows_rcn.unprocessed⟩
 
 theorem unprocessed_ssubset (e : s₁ ↓ₛ s₂) : s₂.unprocessed ⊂ s₁.unprocessed := by
   simp [e.unprocessed_eq, Set.ssubset_iff_subset_ne]
