ReactorModel/Objects/Change.lean
@@ -6,71 +6,71 @@ abbrev Component.Valued.changeType : Component.Valued → Type
 
 namespace Change
 
-protected structure Normal where
+protected structure Normal (ι) where
   cpt   : Component.Valued
-  id    : ID
+  id    : ι
   value : cpt.changeType
 
 opaque Reactor.Class : Type
 
-protected inductive Mutation
-  | connect    (srcPort : ID) (dstPort : ID)
-  | disconnect (srcPort : ID) (dstPort : ID)
+protected inductive Mutation (ι) where
+  | connect    (srcPort : ι) (dstPort : ι)
+  | disconnect (srcPort : ι) (dstPort : ι)
   | create     («class» : Reactor.Class)
-  | delete     (rtr : ID)
+  | delete     (rtr : ι)
 
 end Change
 
-inductive Change
-  | norm  : Change.Normal → Change
-  | «mut» : Change.Mutation → Change
+inductive Change (ι) where
+  | norm  (n : Change.Normal ι)
+  | «mut» (m : Change.Mutation ι)
 
 namespace Change
 
-instance : Coe Change.Normal Change where
+instance : Coe (Change.Normal ι) (Change ι) where
   coe := norm
 
-instance : Coe Change.Mutation Change where
+instance : Coe (Change.Mutation ι) (Change ι) where
   coe := «mut»
 
 @[match_pattern]
-abbrev inp (i : ID) (v : Value) : Change :=
+abbrev inp (i : ι) (v : Value) : Change ι :=
   .norm <| { cpt := .inp, id := i, value := v }
 
 @[match_pattern]
-abbrev out (i : ID) (v : Value) : Change :=
+abbrev out (i : ι) (v : Value) : Change ι :=
   .norm <| { cpt := .out, id := i, value := v }
 
 @[match_pattern]
-abbrev stv (i : ID) (v : Value) : Change :=
+abbrev stv (i : ι) (v : Value) : Change ι :=
   .norm <| { cpt := .stv, id := i, value := v }
 
 @[match_pattern]
-abbrev act (i : ID) (t : Time) (v : Value) : Change :=
+abbrev act (i : ι) (t : Time) (v : Value) : Change ι :=
   .norm <| { cpt := .act, id := i, value := (t, v) }
 
-inductive Targets : Change → Component.Valued → ID → Prop
+inductive Targets : Change ι → Component.Valued → ι → Prop
   | intro : Targets (norm ⟨cpt, i, v⟩) cpt i
 
-theorem Targets.norm_not (h : ¬Targets (norm ⟨c, j, v⟩) cpt i) : cpt ≠ c ∨ i ≠ j := by
+theorem Targets.norm_not {j : ι} (h : ¬Targets (norm ⟨c, j, v⟩) cpt i) : cpt ≠ c ∨ i ≠ j := by
   by_contra hc
   simp [not_or] at hc
   exact hc.left ▸ hc.right ▸ h <| .intro
 
-def target : Change → Option (Component.Valued × ID)
+def target : Change ι → Option (Component.Valued × ι)
   | norm ⟨cpt, i, _⟩ => (cpt, i)
   | «mut» ..         => none
 
-inductive IsNormal : Change → Prop
+inductive IsNormal : Change ι → Prop where
   | intro : IsNormal (norm _)
 
-inductive IsMutation : Change → Prop
+inductive IsMutation : Change ι → Prop where
   | intro : IsMutation («mut» _)
 
-inductive IsPort : Change → Prop
+inductive IsPort : Change ι → Prop where
   | intro : IsPort (prt ..)
 
-inductive IsAction : Change → Prop
+inductive IsAction : Change ι → Prop where
   | intro : IsAction (act ..)
 
 end Change
