ReactorModel/Objects/Reactor/Basic.lean
@@ -2,36 +2,34 @@ import ReactorModel.Objects.Reaction
 
 noncomputable section
 
-abbrev Component.type (rtrType : Type) : Component → Type
-  | .rtr   => rtrType 
-  | .rcn   => Reaction
+abbrev Component.type (α : Type) [Identifiable α] : Component → Type
+  | .rtr   => α
+  | .rcn   => Reaction α✦
   | .val _ => Value
 
--- Note: This approach is similar to how algebras are defined in category theory, where the 
---       `Component` parameter plays the role of the functor over which the algrabra is defined.
-class Reactor (α : Type) where
-  get? : α → (cpt : Component) → (ID ⇀ cpt.type α)   
- 
+class Reactor (α : Type) extends Identifiable α where
+  get? : α → (cpt : Component) → (α✦ ⇀ cpt.type α)
+
 namespace Reactor
 
 notation rtr "{" cpt "}"        => get? rtr cpt
 notation rtr "{" cpt "}{" i "}" => get? rtr cpt i
 
-inductive StrictMember [Reactor α] (cpt : Component) (i : ID) : α → Type
+inductive StrictMember [Reactor α] (cpt : Component) (i) : α → Type
   | final  : (rtr{cpt}{i} = some o) → StrictMember cpt i rtr
   | nested : (rtr₁{.rtr}{j} = some rtr₂) → (StrictMember cpt i rtr₂) → StrictMember cpt i rtr₁
 
 namespace StrictMember
 
-def object [Reactor α] {rtr : α} : (StrictMember cpt i rtr) → cpt.type α
+abbrev object [Reactor α] {rtr : α} {i} : (StrictMember cpt i rtr) → cpt.type α
   | final (o := o) _ => o
   | nested _ m       => m.object
 
 end StrictMember
 
-inductive Member [Reactor α] : (cpt : Component) → (i : cpt.idType) → α → Type 
+inductive Member [Reactor α] : (cpt : Component) → (i : α✦cpt) → α → Type
   | root   : Member .rtr ⊤ rtr
-  | strict : (StrictMember cpt i rtr) → Member cpt i rtr 
+  | strict : (StrictMember cpt i rtr) → Member cpt i rtr
 
 namespace Member
 
@@ -41,26 +39,26 @@ instance : Coe (StrictMember cpt i rtr) (Member cpt i rtr) where
   coe := .strict
 
 @[match_pattern]
-abbrev final (h : rtr{cpt}{i} = some o) : Member cpt i rtr := 
+abbrev final (h : rtr{cpt}{i} = some o) : Member cpt i rtr :=
   StrictMember.final h
 
 @[match_pattern]
-abbrev nested (h : rtr{.rtr}{j} = some rtr') (s : StrictMember cpt i rtr') : Member cpt i rtr := 
+abbrev nested (h : rtr{.rtr}{j} = some rtr') (s : StrictMember cpt i rtr') : Member cpt i rtr :=
   StrictMember.nested h s
 
-def object {rtr : α} : (Member cpt i rtr) → cpt.type α
+abbrev object {rtr : α} : (Member cpt i rtr) → cpt.type α
   | root     => rtr
   | strict s => s.object
 
 end Member
 
--- The relation lifts the notion of a member having an objects to the notion of an identified 
--- component having an object. When `α` is `Hierarchical` there exists at most one objects for any 
--- given identified component. 
-inductive Object [Reactor α] (rtr : α) (cpt : Component) (i : cpt.idType) : cpt.type α → Prop
+-- The relation lifts the notion of a member having an objects to the notion of an identified
+-- component having an object. When `α` is `Hierarchical` there exists at most one objects for any
+-- given identified component.
+inductive Object [Reactor α] (rtr : α) (cpt : Component) (i : α✦cpt) : cpt.type α → Prop
   | intro (m : Member cpt i rtr) : Object rtr cpt i m.object
 
-def RootEqualUpTo [Reactor α] (cpt : Component) (i : ID) (rtr₁ rtr₂ : α) : Prop :=
+def RootEqualUpTo [Reactor α] (cpt : Component) (i : α✦) (rtr₁ rtr₂ : α) : Prop :=
   ∀ {c j}, (c ≠ cpt ∨ j ≠ i) → rtr₁{c}{j} = rtr₂{c}{j}
 
 notation rtr₁ " ≃[" cpt "][" i "] " rtr₂ => RootEqualUpTo cpt i rtr₁ rtr₂
