ReactorModel/Objects/Reactor/Finite.lean
@@ -8,7 +8,7 @@ namespace Reactor
 class Finite (α) [Hierarchical α] where
   fin : ∀ (rtr : α) (cpt : Component), rtr[cpt].Finite
 
-def Finite.ids [Hierarchical α] [Finite α] (rtr : α) (cpt : Component) : List cpt.idType :=
+def Finite.ids [Hierarchical α] [Finite α] (rtr : α) (cpt : Component) : List α✦cpt :=
   (fin rtr cpt).toFinset.toList
 
 namespace Reactor
