ReactorModel/Objects/Reactor/Updatable.lean
@@ -7,7 +7,7 @@ variable [Reactor α]
 -- Note: Without ID-uniqueness this can be satisfied by updating exactly one of the occurrences of
 --       the target. Since we have a choice of which target we update, this type isn't a `Prop`.
 --       (We need to be able to eliminate into `Type` in `Member.fromLawfulUpdate`).
-inductive LawfulMemUpdate (cpt : Component.Valued) (i : ID) (v : Value) : α → α → Type
+inductive LawfulMemUpdate (cpt : Component.Valued) (i) (v : Value) : α → α → Type
   | final :
     (rtr₁ ≃[cpt][i] rtr₂) → (rtr₁{cpt}{i} = some o) → (rtr₂{cpt}{i} = v) →
     LawfulMemUpdate cpt i v rtr₁ rtr₂
@@ -16,12 +16,12 @@ inductive LawfulMemUpdate (cpt : Component.Valued) (i : ID) (v : Value) : α →
     (LawfulMemUpdate cpt i v n₁ n₂) → LawfulMemUpdate cpt i v rtr₁ rtr₂
 
 -- Note: This isn't a `Prop` because of the explanation on `LawfulMemUpdate`.
-inductive LawfulUpdate (cpt : Component.Valued) (i : ID) (v : Value) (rtr₁ rtr₂ : α)
+inductive LawfulUpdate (cpt : Component.Valued) (i) (v : Value) (rtr₁ rtr₂ : α)
   | update (u : LawfulMemUpdate cpt i v rtr₁ rtr₂)
   | notMem (h : IsEmpty <| Member cpt i rtr₁) (eq : rtr₁ = rtr₂)
 
 class Updatable (α) extends Reactor α where
-  update : α → (cpt : Component.Valued) → ID → Value → α
+  update : α → (cpt : Component.Valued) → α✦ → Value → α
 
 class LawfulUpdatable (α) extends Updatable α where
   lawful : ∀ rtr cpt i v, LawfulUpdate cpt i v rtr (update rtr cpt i v)
