ReactorModel/Execution/Dependency.lean
@@ -4,27 +4,27 @@ open Reactor
 
 variable [Hierarchical α]
 
--- About the `↔`-condition in `prio`:  We want to establish a dependency between mutations with 
+-- About the `↔`-condition in `prio`:  We want to establish a dependency between mutations with
 -- priorities as well normal reactions with priorities, but not between normal reactions and
 -- mutations. Otherwise a normal reaction might take precedence over a mutation. Also the precedence
 -- of mutations over normal reactions is handled by `mutNorm`, so this would potentially create a
 -- redundancy.
 --
--- Note: `Dependency rtr i₁ i₂` means that in `i₁` must occur before `i₂`. 
-inductive Dependency (rtr : α) : ID → ID → Prop
-  | prio : 
-    (rtr[.rtr][i] = some con) → (con{.rcn}{i₁} = some rcn₁) → (con{.rcn}{i₂} = some rcn₂) → 
+-- Note: `Dependency rtr i₁ i₂` means that in `i₁` must occur before `i₂`.
+inductive Dependency (rtr : α) : α✦ → α✦ → Prop
+  | prio :
+    (rtr[.rtr][i] = some con) → (con{.rcn}{i₁} = some rcn₁) → (con{.rcn}{i₂} = some rcn₂) →
     (rcn₁.Mutates ↔ rcn₂.Mutates) → (rcn₁.prio > rcn₂.prio) → Dependency rtr i₁ i₂
-  | depOverlap {d : Reaction.Dependency} :
-    (rtr[.rcn][i₁] = some rcn₁) → (rtr[.rcn][i₂] = some rcn₂) → (d ∈ rcn₁.deps .out) → 
+  | depOverlap {d : Reaction.Dependency α✦} :
+    (rtr[.rcn][i₁] = some rcn₁) → (rtr[.rcn][i₂] = some rcn₂) → (d ∈ rcn₁.deps .out) →
     (d ∈ rcn₂.deps .in) → (d.cpt ≠ .stv) → Dependency rtr i₁ i₂
-  | mutNorm : 
-    (rtr[.rtr][i] = some con) → (con{.rcn}{iₘ} = some m) → (con{.rcn}{iₙ} = some n) → (m.Mutates) → 
+  | mutNorm :
+    (rtr[.rtr][i] = some con) → (con{.rcn}{iₘ} = some m) → (con{.rcn}{iₙ} = some n) → (m.Mutates) →
     (n.Normal) → Dependency rtr iₘ iₙ
   | mutNest :
-    (rtr[.rtr][i] = some rtr₁) → (rtr₁{.rtr}{j} = some rtr₂) → (rtr₁{.rcn}{iₘ} = some m) → 
+    (rtr[.rtr][i] = some rtr₁) → (rtr₁{.rtr}{j} = some rtr₂) → (rtr₁{.rcn}{iₘ} = some m) →
     (m.Mutates) → (iᵣ ∈ rtr₂{.rcn}) → Dependency rtr iₘ iᵣ
-  | trans : 
+  | trans :
     Dependency rtr i₁ i₂ → Dependency rtr i₂ i₃ → Dependency rtr i₁ i₃
 
 notation i₁ " <[" rtr "] " i₂ => Dependency rtr i₁ i₂
