ReactorModel/Objects/Reactor/Proper.lean
@@ -6,23 +6,23 @@ import ReactorModel.Objects.Reactor.Updatable
 namespace Reactor
 namespace Wellformed
 
--- `ValidDependency rtr rk dk d` means that in reactor `rtr`, reactions of kind `rk` can have `d` as 
--- a valid dependency target of kind `dk`. For example `ValidDependency rtr .mut .out (.port .in i)` 
--- states that mutations can specify the input port identified by `i` as effect and 
--- `ValidDependency rtr .norm .in (.action i)` states that normal reactions can specify the action 
+-- `ValidDependency rtr rk dk d` means that in reactor `rtr`, reactions of kind `rk` can have `d` as
+-- a valid dependency target of kind `dk`. For example `ValidDependency rtr .mut .out (.port .in i)`
+-- states that mutations can specify the input port identified by `i` as effect and
+-- `ValidDependency rtr .norm .in (.action i)` states that normal reactions can specify the action
 -- identified by `i` as source.
-inductive ValidDependency [Reactor α] (rtr : α) : 
-    Reaction.Kind → Kind → Reaction.Dependency → Prop
-  | inp       : (i ∈ rtr{.inp})                             → ValidDependency _ _     .in  ⟨.inp, i⟩   
-  | out       : (i ∈ rtr{.out})                             → ValidDependency _ _     .out ⟨.out, i⟩   
-  | stv       : (i ∈ rtr{.stv})                             → ValidDependency _ _     _    ⟨.stv, i⟩  
+inductive ValidDependency [Reactor α] (rtr : α) :
+    Reaction.Kind → Kind → Reaction.Dependency _ → Prop where
+  | inp       : (i ∈ rtr{.inp})                             → ValidDependency _ _     .in  ⟨.inp, i⟩
+  | out       : (i ∈ rtr{.out})                             → ValidDependency _ _     .out ⟨.out, i⟩
+  | stv       : (i ∈ rtr{.stv})                             → ValidDependency _ _     _    ⟨.stv, i⟩
   | act       : (i ∈ rtr{.act})                             → ValidDependency _ _     _    ⟨.act, i⟩
   | nestedIn  : (rtr{.rtr}{j} = some con) → (i ∈ con{.inp}) → ValidDependency _ _     .out ⟨.inp, i⟩
-  | nestedOut : (rtr{.rtr}{j} = some con) → (i ∈ con{.out}) → ValidDependency _ .norm .in  ⟨.out, i⟩ 
+  | nestedOut : (rtr{.rtr}{j} = some con) → (i ∈ con{.out}) → ValidDependency _ .norm .in  ⟨.out, i⟩
 
--- Note: This proposition is only meaningful under the condition that `rcn₁` and `rcn₂` live in the 
+-- Note: This proposition is only meaningful under the condition that `rcn₁` and `rcn₂` live in the
 --       same reactor.
-inductive NeedOrderedPriority (rcn₁ rcn₂ : Reaction) : Prop
+inductive NeedOrderedPriority (rcn₁ rcn₂ : Reaction ι) : Prop
   | overlap (h₁ : d ∈ rcn₁.deps .out) (h₂ : d ∈ rcn₂.deps .out)
   | hazard (h₁ : ⟨.stv, s⟩ ∈ rcn₁.deps k₁) (h₂ : ⟨.stv, s⟩ ∈ rcn₂.deps k₂) (ho : k₁ = .out ∨ k₂ = .out)
   | mutation (h₁ : rcn₁.Mutates) (h₂ : rcn₂.Mutates)
@@ -32,13 +32,13 @@ end Wellformed
 open Wellformed
 
 structure Wellformed [idx : Hierarchical α] (rtr : α) : Prop where
-  unique_inputs : (rtr[.rcn][i₁] = some rcn₁) → (rtr[.rcn][i₂] = some rcn₂) → (i₁ ≠ i₂) → 
-                  (⟨.inp, i⟩ ∈ rcn₁.deps .out) → (⟨.inp, i⟩ ∉ rcn₂.deps .out)  
-  ordered_prio  : (rtr[.rtr][i] = some con) → (con{.rcn}{i₁} = some rcn₁) → 
-                  (con{.rcn}{i₂} = some rcn₂) → (i₁ ≠ i₂) → (NeedOrderedPriority rcn₁ rcn₂) → 
+  unique_inputs : (rtr[.rcn][i₁] = some rcn₁) → (rtr[.rcn][i₂] = some rcn₂) → (i₁ ≠ i₂) →
+                  (⟨.inp, i⟩ ∈ rcn₁.deps .out) → (⟨.inp, i⟩ ∉ rcn₂.deps .out)
+  ordered_prio  : (rtr[.rtr][i] = some con) → (con{.rcn}{i₁} = some rcn₁) →
+                  (con{.rcn}{i₂} = some rcn₂) → (i₁ ≠ i₂) → (NeedOrderedPriority rcn₁ rcn₂) →
                   (rcn₁.prio < rcn₂.prio ∨ rcn₂.prio < rcn₁.prio)
-  valid_deps    : (rtr[.rtr][i] = some con) → (con{.rcn}{j} = some rcn) → (d ∈ rcn.deps k) → 
-                  (ValidDependency con rcn.kind k d) 
+  valid_deps    : (rtr[.rtr][i] = some con) → (con{.rcn}{j} = some rcn) → (d ∈ rcn.deps k) →
+                  (ValidDependency con rcn.kind k d)
 
 class Proper (α) extends Extensional α, Hierarchical α, WellFounded α, LawfulUpdatable α where
   wellformed : ∀ rtr : α, Wellformed rtr (idx := toHierarchical)
