ReactorModel/Objects/Reactor/Theorems/Extensional.lean
@@ -4,12 +4,12 @@ namespace Reactor
 
 variable [Extensional α] {rtr₁ : α}
 
-theorem RootEqualUpTo.ext (e : rtr₁ ≃[cpt][i] rtr₂) (h : rtr₁{cpt}{i} = rtr₂{cpt}{i}) : 
+theorem RootEqualUpTo.ext (e : rtr₁ ≃[cpt][i] rtr₂) (h : rtr₁{cpt}{i} = rtr₂{cpt}{i}) :
     rtr₁ = rtr₂ := by
   ext1; ext1 c; ext1 j
   by_cases hc : c = cpt <;> by_cases hj : j = i
-  · exact hc ▸ hj ▸ h 
-  · exact hc ▸ e (.inr hj) 
+  · exact hc ▸ hj ▸ h
+  · exact hc ▸ e (.inr hj)
   · exact e (.inl hc)
   · exact e (.inl hc)
 
